

# Loop Invariants and Insertion-sort

## COMS10018 - Algorithms

Dr Christian Konrad

# Loop Invariants

**Definition:** A *loop invariant* is a property  $P$  that, if true before iteration  $i$ , it is also true before iteration  $i + 1$

**Example:**

Computing the maximum

**Invariant:** Before iteration  $i$ :  
 $m = \max\{A[j] : 0 \leq j < i\}$

```
Require: Array of  $n$  positive integers  $A$   
 $m \leftarrow A[0]$   
for  $i = 1, \dots, n - 1$  do  
    if  $A[i] > m$  then  
         $m \leftarrow A[i]$   
return  $m$ 
```

**Proof:** Let  $m_i$  be the value of  $m$  before iter.  $i$  ( $\rightarrow m_1 = A[0]$ ).

- *Base case.*  $i = 1$ :  $m_1 = A[0] = \max\{A[j] : 0 \leq j < 1\}$  ✓

- *Induction step.*

**Case**  $A[i] > m_i$ :  $m_{i+1} = A[i] > m_i = \max\{A[j] : 0 \leq j < i\} \Rightarrow m_{i+1} = \max\{A[j] : 0 \leq j < i + 1\}$

**Case**  $A[i] \leq m_i$ :  $m_{i+1} = m_i = \max\{A[j] : 0 \leq j < i\} = \max\{A[j] : 0 \leq j < i + 1\}$  ✓

# Loop Invariants - More Formally

## Main Parts:

- **Initialization:** It is true prior to the first iteration of the loop.  
before iteration  $i = 1 : m = A[0] = \max\{A[j] : j < 1\} \checkmark$
- **Maintenance:** If it is true before an iteration of the loop, it remains true before the next iteration.  
before iteration  $i > 1 : m = \max\{A[j] : j < i\} \checkmark$
- **Termination:** When the loop terminates, the invariant gives us a useful property that helps show that the algorithm is correct.  
At the end of the loop, i.e., after iteration  $n - 1$  (or before a virtual iteration  $n$ )  $m = m_n = \max\{A[j] : j < n\} \checkmark$

# Example

```
Require:  $n$  integer  
   $s \leftarrow 1$   
  for  $j = 2, \dots, n$  do  
     $s \leftarrow s \cdot j$   
  return  $s$ 
```

**Invariant:** At beginning of iteration  $j$ :  $s = (j - 1)!$

- ① Let  $s_j$  be the value of  $s$  prior to iteration  $j$
- ② **Initialization:**  $s_2 = 1 = (2 - 1)! \checkmark$
- ③ **Maintenance:**  $s_{j+1} = s_j \cdot j = (j - 1)! \cdot j = j! \checkmark$
- ④ **Termination:** After iteration  $n$ , i.e., before iteration  $n + 1$ , the value of  $s$  is  $s_{n+1} = (n + 1 - 1)! = n! \checkmark$

Algorithm computes the factorial function

# Example: Insertion Sort

## Sorting Problem

- **Input:** An array  $A$  of  $n$  numbers
- **Output:** A reordering of  $A$  s.t.  $A[0] \leq A[1] \leq \dots \leq A[n-1]$

```
Require: Array  $A$  of  $n$  numbers  
for  $j = 1, \dots, n-1$  do  
     $v \leftarrow A[j]$   
     $i \leftarrow j-1$   
    while  $i \geq 0$  and  $A[i] > v$  do  
         $A[i+1] \leftarrow A[i]$   
         $i \leftarrow i-1$   
     $A[i+1] \leftarrow v$ 
```

INSERTION-SORT

## Example:

```
Require: Array  $A$  of  $n$  numbers  
for  $j = 1, \dots, n - 1$  do  
     $v \leftarrow A[j]$   
     $i \leftarrow j - 1$   
    while  $i \geq 0$  and  $A[i] > v$  do  
         $A[i + 1] \leftarrow A[i]$   
         $i \leftarrow i - 1$   
     $A[i + 1] \leftarrow v$ 
```

0	1	2	3	4	$j = 5$
1	3	7	8	9	15

# Loop Invariant of Insertion-sort

```
for  $j = 1, \dots, n - 1$  do  
     $v \leftarrow A[j]$   
     $i \leftarrow j - 1$   
    while  $i \geq 0$  and  $A[i] > v$  do  
         $A[i + 1] \leftarrow A[i]$   
         $i \leftarrow i - 1$   
     $A[i + 1] \leftarrow v$ 
```

**Loop Invariant:** At beginning of iteration  $j$  of the outer **for** loop, the subarray  $A[0, j - 1]$  consists of the elements originally in  $A[0, j - 1]$ , but in sorted order

- **Initialization:**  $j = 1$ : subarray  $A[0]$  is sorted ✓
- **Maintenance:** *Informally*, element  $A[j]$  is inserted at the right place within  $A[0, j]$ . A formal argument would require another loop invariant for the inner loop. ✓
- **Termination:** After iteration  $j = n - 1$  (i.e., before iteration  $j = n$ ) the loop invariant states that  $A$  is sorted. ✓

# Worst-case Runtime of Insertion-sort

## Worst-case Runtime:

- We have two nested loops
- The outer loop goes from  $j = 1$  to  $j = n - 1$
- The inner loop goes from  $i = j - 1$  down to  $i = 0$  in worst case
- All other operations take time  $O(1)$ . Hence:

$$\sum_{j=1}^{n-1} j \cdot O(1) = O(1) \sum_{j=1}^{n-1} j = O(1) \frac{n(n-1)}{2} = O(1)(n^2 - n) = O(n^2).$$

## Best-case Runtime: $O(n)$

E.g., if input is already sorted